Move some reusable code to proper position

coq/proof/InvState.v
@@ -55,6 +55,15 @@ Module Unary.
   Definition update_both f x :=
     update_ghost f (update_previous f x).
 
+  Definition filter
+             (preserved: Exprs.Tag.t * id -> bool)
+             (inv: t): t :=
+    update_ghost
+      (filter_AL_atom (preserved <*> (pair Exprs.Tag.ghost)))
+      (update_previous
+         (filter_AL_atom (preserved <*> (pair Exprs.Tag.previous)))
+         inv).
+
   Definition sem_tag (st:State) (invst:t) (tag:Tag.t): GVsMap :=
     match tag with
     | Tag.physical => st.(EC).(Locals)
@@ -169,6 +178,139 @@ Module Unary.
       end
     end.
 
+  Lemma filter_subset_idT st_unary f id invst_unary val
+        (VAL_SUBSET: (sem_idT st_unary (filter f invst_unary) id = Some val)):
+    <<VAL: (sem_idT st_unary invst_unary id = Some val)>>.
+  Proof.
+    red.
+    unfold sem_idT in *.
+    unfold filter, filter_AL_atom in *.
+    unfold update_ghost, update_previous in *. ss.
+    unfold sem_tag in *. ss.
+    destruct id. rename i0 into id. ss.
+    destruct invst_unary. ss.
+    destruct t0; ss.
+    - exploit (@lookup_AL_filter_some GenericValue); eauto.
+    - exploit (@lookup_AL_filter_some GenericValue); eauto.
+  Qed.
+
+  Lemma filter_subset_valueT conf_unary st_unary f vt invst_unary val
+        (VAL_SUBSET: (sem_valueT conf_unary st_unary
+                                 (filter f invst_unary) vt = Some val)):
+    <<VAL: (sem_valueT conf_unary st_unary invst_unary vt = Some val)>>.
+  Proof.
+    red.
+    destruct vt; ss.
+    exploit filter_subset_idT; eauto.
+  Qed.
+
+  Lemma filter_subset_list_valueT conf_unary st_unary f vts invst_unary val
+        (VAL_SUBSET: (sem_list_valueT conf_unary st_unary
+                                      (filter f invst_unary) vts = Some val)):
+    <<VAL: (sem_list_valueT conf_unary st_unary invst_unary vts = Some val)>>.
+  Proof.
+    red.
+    generalize dependent val.
+    induction vts; i; ss.
+    destruct a; ss.
+    Ltac exploit_with H x :=
+      (exploit H; [exact x|]; eauto; ii; des).
+    des_ifs; ss;
+      (all_once exploit_with filter_subset_valueT);
+      (exploit IHvts; eauto; ii; des); clarify.
+  Qed.
+
+  Lemma filter_subset_expr conf_unary st_unary f expr invst_unary val
+        (VAL_SUBSET: (sem_expr conf_unary st_unary
+                               (filter f invst_unary) expr = Some val)):
+    <<VAL: (sem_expr conf_unary st_unary invst_unary expr = Some val)>>.
+  Proof.
+    red.
+    Ltac exploit_filter_subset_with x :=
+      match (type of x) with
+      | (sem_valueT _ _ _ _ = Some _) =>
+        (exploit filter_subset_valueT; [exact x|]; eauto; ii; des)
+      | (sem_list_valueT _ _ _ _ = Some _) =>
+        (exploit filter_subset_list_valueT; [exact x|]; eauto; ii; des)
+      end.
+    Time destruct expr; ss;
+      des_ifs; ss; (all_once exploit_filter_subset_with); clarify.
+  (* exploit_with: Finished transaction in 25.39 secs (25.194u,0.213s) (successful) *)
+  (* exploit_with_fast: Finished transaction in 7.575 secs (7.536u,0.044s) (successful) *)
+  Qed.
+
+  Lemma filter_preserved_valueT
+        conf_unary st_unary invst_unary vt val f
+        (VAL: sem_valueT conf_unary st_unary invst_unary vt = Some val)
+        (PRESERVED: (sflib.is_true (List.forallb f (Exprs.ValueT.get_idTs vt)))):
+    <<VAL: sem_valueT conf_unary st_unary (filter f invst_unary) vt = Some val>>.
+  Proof.
+    red.
+    destruct vt; ss.
+    repeat (des_bool; des). clear PRESERVED0.
+    unfold sem_idT in *.
+    destruct x; ss.
+    unfold filter.
+    destruct invst_unary; ss.
+    unfold compose in *.
+    unfold Exprs.Tag.t in *. (* TODO doing left unfold is a bit annoying *)
+    destruct t0; ss; rewrite lookup_AL_filter_spec in *; des_ifs.
+  Qed.
+
+  Lemma filter_preserved_list_valueT
+        conf_unary st_unary invst_unary vts val f
+        (VAL: sem_list_valueT conf_unary st_unary invst_unary vts = Some val)
+        (PRESERVED: sflib.is_true (List.forallb
+                                     (fun x => (List.forallb f (Exprs.ValueT.get_idTs x)))
+                                     (List.map snd vts))):
+    <<VAL: sem_list_valueT conf_unary st_unary (filter f invst_unary) vts = Some val>>.
+  Proof.
+    generalize dependent PRESERVED.
+    generalize dependent val.
+    induction vts; ii; ss; red.
+    destruct a; ss.
+    repeat (des_bool; des).
+    des_ifs; ss.
+    - (exploit filter_preserved_valueT; [exact Heq1| |]; eauto; ii; des).
+      exploit IHvts; eauto; []; ii; des.
+      clarify.
+    - (exploit filter_preserved_valueT; [exact Heq1| |]; eauto; ii; des).
+      clarify.
+      exploit IHvts; eauto; []; ii; des.
+      clarify.
+    - (exploit filter_preserved_valueT; [exact Heq0| |]; eauto; ii; des).
+      exploit IHvts; eauto; []; ii; des.
+      clarify.
+  Qed.
+
+  Lemma filter_preserved_expr
+        conf_unary st_unary invst_unary expr val f
+        (VAL: sem_expr conf_unary st_unary invst_unary expr = Some val)
+        (PRESERVED: List.forallb f (Exprs.Expr.get_idTs expr)):
+    <<VAL: sem_expr conf_unary st_unary (filter f invst_unary) expr = Some val>>.
+  Proof.
+    red.
+    unfold Exprs.Expr.get_idTs in *.
+    eapply forallb_filter_map in PRESERVED. des.
+    unfold is_true in PRESERVED. (* des_bool should kill it!!!!!!! KILL ALL is_true *)
+
+    Ltac exploit_filter_preserved_with x :=
+      match (type of x) with
+      | (sem_valueT _ _ (filter _ _) _ = _) => fail 1
+      | (sem_list_valueT _ _ (filter _ _) _ = _) => fail 1
+      (* Above is REQUIRED in order to prevent inf loop *)
+      | (sem_valueT _ _ _ _ = Some _) =>
+        (exploit filter_preserved_valueT; [exact x| |]; eauto; ii; des)
+      | (sem_list_valueT _ _ _ _ = Some _) =>
+        (exploit filter_preserved_list_valueT; [exact x| |]; eauto; ii; des)
+      end.
+
+    Time destruct expr; ss;
+      repeat (des_bool; des); des_ifs; clarify;
+        (all_once exploit_filter_subset_with); clarify;
+          (all_once exploit_filter_preserved_with); clarify.
+  Qed.
+
   Definition sem_lessdef (conf:Config) (st:State) (invst:t) (es:ExprPair.t): Prop :=
     forall val1 (VAL1: sem_expr conf st invst es.(fst) = Some val1),
     exists val2,
@@ -247,6 +389,63 @@ Module Unary.
       (PRIVATE: IdTSet.For_all (sem_private conf st invst invmem.(InvMem.Unary.private)) inv.(Invariant.private))
   .
 
+  Lemma incl_implies_preserved
+        conf st invst0 expr val inv
+        (preserved: _ -> bool)
+        (PRESERVED: forall id (ID: In id (Hints.Invariant.get_idTs_unary inv)), preserved id)
+        (VAL: sem_expr conf st invst0 expr = Some val)
+        (INCL: incl (Exprs.Expr.get_idTs expr) (Hints.Invariant.get_idTs_unary inv)):
+    <<PRESERVED: sem_expr conf st (filter preserved invst0) expr = Some val>>.
+  Proof.
+    eapply filter_preserved_expr; eauto. apply forallb_forall. i.
+    apply PRESERVED. apply INCL. ss.
+  Qed.
+
+  (* TODO put this in FSetExtra *)
+  Lemma In_list {A} (f: Exprs.ExprPair.t -> list A) x xs
+        (IN: Exprs.ExprPairSet.In x xs):
+    <<IN: List.incl (f x) (List.concat (List.map f (Exprs.ExprPairSet.elements xs)))>>.
+  Proof.
+    red.
+    exploit Exprs.ExprPairSetFacts.elements_iff; eauto; []; ii; des.
+    specialize (H IN). clear IN.
+    specialize (H1 H).
+    exploit InA_iff_In; eauto. ii; des.
+    specialize (H2 H). clear H3.
+    assert(G: In (f x) (List.map f (Exprs.ExprPairSet.elements xs))).
+    { eapply In_map; eauto. }
+    exploit (@In_concat A Exprs.ExprPair.t (list A)); eauto.
+  Qed.
+
+  Lemma filter_spec
+        conf st invst invmem inv
+        (preserved: _ -> bool)
+        (PRESERVED: forall id (ID: In id (Hints.Invariant.get_idTs_unary inv)), preserved id)
+        (STATE: sem conf st invst invmem inv):
+    sem conf st (filter preserved invst) invmem inv.
+  Proof.
+    inv STATE. econs.
+    - ii.
+      exploit filter_subset_expr; eauto. i. des.
+      exploit LESSDEF; eauto. i. des.
+      exploit incl_implies_preserved; eauto.
+      eapply incl_tran; [|eapply incl_tran].
+      + apply incl_appr. apply incl_refl.
+      + eapply In_list in H. des. refine H.
+      + unfold Hints.Invariant.get_idTs_unary.
+        apply incl_appl. apply incl_refl.
+    - inv NOALIAS. econs; i.
+      + eapply DIFFBLOCK; eauto.
+        * eapply filter_subset_valueT; eauto.
+        * eapply filter_subset_valueT; eauto.
+      + eapply NOALIAS0; eauto.
+        * eapply filter_subset_valueT; eauto.
+        * eapply filter_subset_valueT; eauto.
+    - ii. exploit UNIQUE; eauto. i. inv H0.
+      econs; eauto.
+    - ii. exploit PRIVATE; eauto.
+      eapply filter_subset_idT; eauto.
+  Qed.
 
   Lemma sem_empty
         conf st invst invmem inv
@@ -286,6 +485,11 @@ Module Rel.
 
   Definition update_both f x :=
     update_src f (update_tgt f x).
+
+  Definition filter
+             (preserved: Exprs.Tag.t * id -> bool)
+             (inv: t): t :=
+    update_both (Unary.filter preserved) inv.
 
   Definition sem_inject (st_src st_tgt:State) (invst:t) (inject:meminj) (id:IdT.t): Prop :=
     forall val_src (VAL_SRC: Unary.sem_idT st_src invst.(src) id = Some val_src),
