coq/proof/SoundReduceMaydiff.v
@@ -91,258 +91,28 @@ Qed.
  * otherwise: none
  *)
 
-Definition clear_locals
-           (preserved: id -> bool)
-           (locals: GVsMap): GVsMap :=
-  filter_AL_atom (preserved) locals.
-
-Definition clear_unary
-           (preserved: Exprs.Tag.t * id -> bool)
-           (inv: InvState.Unary.t): InvState.Unary.t :=
-  InvState.Unary.update_ghost
-    (clear_locals (fun id => preserved (Exprs.Tag.ghost, id)))
-    (InvState.Unary.update_previous
-       (clear_locals (fun id => preserved (Exprs.Tag.previous, id)))
-       inv).
-
-Lemma clear_locals_spec
-      pred gvs i:
-  lookupAL _ (clear_locals pred gvs) i =
-  if pred i
-  then lookupAL _ gvs i
-  else None.
-Proof.
-  unfold clear_locals. destruct (pred i) eqn:PRED.
-  - apply lookup_AL_filter_true. ss.
-  - apply lookup_AL_filter_false. ss.
-Qed.
-
-Definition clear_rel
-           (preserved: Exprs.Tag.t * id -> bool)
-           (inv: InvState.Rel.t): InvState.Rel.t :=
-  InvState.Rel.update_both (clear_unary preserved) inv.
-
-Lemma clear_unary_subset_idT st_unary f id invst_unary val
-      (VAL_SUBSET: (InvState.Unary.sem_idT
-                   st_unary (clear_unary f invst_unary) id =
-                 Some val)):
-  <<VAL: (InvState.Unary.sem_idT st_unary invst_unary id =
-          Some val)>>.
-Proof.
-  red.
-  unfold InvState.Unary.sem_idT in *.
-  unfold clear_unary, clear_locals in *.
-  unfold InvState.Unary.update_ghost, InvState.Unary.update_previous in *. ss.
-  unfold InvState.Unary.sem_tag in *. ss.
-  destruct id. rename i0 into id. ss.
-  destruct invst_unary. ss.
-  destruct t; ss.
-  - exploit (@lookup_AL_filter_some GenericValue); eauto.
-  - exploit (@lookup_AL_filter_some GenericValue); eauto.
-Qed.
-
-Lemma clear_unary_subset_valueT conf_unary st_unary f vt invst_unary val
-      (VAL_SUBSET: (InvState.Unary.sem_valueT conf_unary
-                   st_unary (clear_unary f invst_unary) vt =
-                 Some val)):
-  <<VAL: (InvState.Unary.sem_valueT conf_unary st_unary invst_unary vt =
-          Some val)>>.
-Proof.
-  red.
-  destruct vt; ss.
-  exploit clear_unary_subset_idT; eauto.
-Qed.
-
-Lemma clear_unary_subset_list_valueT conf_unary st_unary f vts invst_unary val
-      (VAL_SUBSET: (InvState.Unary.sem_list_valueT conf_unary
-                   st_unary (clear_unary f invst_unary) vts =
-                 Some val)):
-  <<VAL: (InvState.Unary.sem_list_valueT conf_unary st_unary invst_unary vts =
-          Some val)>>.
-Proof.
-  red.
-  generalize dependent val.
-  induction vts; i; ss.
-  destruct a; ss.
-  Ltac exploit_with H x :=
-    (exploit H; [exact x|]; eauto; ii; des).
-  des_ifs; ss; (all_once exploit_with clear_unary_subset_valueT); (exploit IHvts; eauto; ii; des); clarify.
-Qed.
-
-Lemma clear_unary_subset_expr conf_unary st_unary f expr invst_unary val
-      (VAL_SUBSET: (InvState.Unary.sem_expr conf_unary
-                   st_unary (clear_unary f invst_unary) expr =
-                 Some val)):
-  <<VAL: (InvState.Unary.sem_expr conf_unary st_unary invst_unary expr =
-          Some val)>>.
-Proof.
-  red.
-  Ltac exploit_clear_unary_subset_with x :=
-    match (type of x) with
-    | (InvState.Unary.sem_valueT _ _ _ _ = Some _) =>
-      (exploit clear_unary_subset_valueT; [exact x|]; eauto; ii; des)
-    | (InvState.Unary.sem_list_valueT _ _ _ _ = Some _) =>
-      (exploit clear_unary_subset_list_valueT; [exact x|]; eauto; ii; des)
-    end.
-  Time destruct expr; ss;
-    des_ifs; ss; (all_once exploit_clear_unary_subset_with); clarify.
-  (* exploit_with: Finished transaction in 25.39 secs (25.194u,0.213s) (successful) *)
-  (* exploit_with_fast: Finished transaction in 7.575 secs (7.536u,0.044s) (successful) *)
-Qed.
-
 Lemma reduce_maydiff_preserved_sem_idT st_src st_tgt
       invst inv id val_src val_tgt
   (VAL_SRC: InvState.Unary.sem_idT st_src
-              (clear_unary (reduce_maydiff_preserved inv) (InvState.Rel.src invst)) id =
+              (InvState.Unary.filter (reduce_maydiff_preserved inv) (InvState.Rel.src invst)) id =
             Some val_src)
   (VAL_TGT: InvState.Unary.sem_idT st_tgt (InvState.Rel.tgt invst) id = Some val_tgt):
   <<VAL_TGT: InvState.Unary.sem_idT st_tgt
-    (clear_unary (reduce_maydiff_preserved inv) (InvState.Rel.tgt invst)) id = Some val_tgt>>.
+    (InvState.Unary.filter (reduce_maydiff_preserved inv) (InvState.Rel.tgt invst)) id = Some val_tgt>>.
 Proof.
   destruct id. rename i0 into id.
   unfold InvState.Unary.sem_idT in *. ss.
   unfold InvState.Unary.sem_tag in *. ss.
-  remember (fun id0 : LLVMsyntax.id => reduce_maydiff_preserved
-                                         inv (Exprs.Tag.previous, id0)) as fnc.
+  unfold compose in *.
   destruct t; ss.
   - rewrite <- VAL_TGT.
-    rewrite clear_locals_spec in *.
+    rewrite lookup_AL_filter_spec in *.
+    rewrite lookup_AL_filter_spec in VAL_SRC. (* WHY SHOULD I WRITE IT ONCE AGAIN?? *)
     des_ifs.
   - rewrite <- VAL_TGT.
-    rewrite clear_locals_spec in *.
+    rewrite lookup_AL_filter_spec in *.
+    rewrite lookup_AL_filter_spec in VAL_SRC. (* WHY SHOULD I WRITE IT ONCE AGAIN?? *)
     des_ifs.
-Qed.
-
-(* TODO put this in FSetExtra *)
-Lemma In_list {A} (f: Exprs.ExprPair.t -> list A) x xs
-      (IN: Exprs.ExprPairSet.In x xs):
-  <<IN: List.incl (f x) (List.concat (List.map f (Exprs.ExprPairSet.elements xs)))>>.
-Proof.
-  red.
-  exploit Exprs.ExprPairSetFacts.elements_iff; eauto; []; ii; des.
-  specialize (x1 IN). clear x0.
-  exploit InA_iff_In; eauto. ii; des.
-  specialize (x2 x1). clear x0. clear x1.
-  assert(G: In (f x) (List.map f (Exprs.ExprPairSet.elements xs))).
-  { eapply In_map; eauto. }
-  exploit (@In_concat A Exprs.ExprPair.t (list A)); eauto.
-Qed.
-
-Lemma clear_unary_preserved_valueT
-      conf_unary st_unary invst_unary vt val f
-      (VAL: InvState.Unary.sem_valueT conf_unary st_unary invst_unary vt = Some val)
-      (PRESERVED: (sflib.is_true (List.forallb f (Exprs.ValueT.get_idTs vt)))):
-  <<VAL: InvState.Unary.sem_valueT conf_unary st_unary (clear_unary f invst_unary) vt = Some val>>.
-Proof.
-  red.
-  destruct vt; ss.
-  repeat (des_bool; des). clear PRESERVED0.
-  unfold InvState.Unary.sem_idT in *.
-  destruct x; ss.
-  unfold clear_unary.
-  destruct invst_unary; ss.
-  unfold Exprs.Tag.t in *. (* TODO doing left unfold is a bit annoying *)
-  destruct t; ss; rewrite clear_locals_spec in *; des_ifs.
-Qed.
-
-Lemma clear_unary_preserved_list_valueT
-      conf_unary st_unary invst_unary vts val f
-      (VAL: InvState.Unary.sem_list_valueT conf_unary st_unary invst_unary vts = Some val)
-      (PRESERVED: sflib.is_true (List.forallb
-                     (fun x => (List.forallb f (Exprs.ValueT.get_idTs x)))
-                     (List.map snd vts))):
-  <<VAL: InvState.Unary.sem_list_valueT conf_unary st_unary (clear_unary f invst_unary) vts = Some val>>.
-Proof.
-  generalize dependent PRESERVED.
-  generalize dependent val.
-  induction vts; ii; ss; red.
-  destruct a; ss.
-  repeat (des_bool; des).
-  des_ifs; ss.
-  - (exploit clear_unary_preserved_valueT; [exact Heq1| |]; eauto; ii; des).
-    exploit IHvts; eauto; []; ii; des.
-    clarify.
-  - (exploit clear_unary_preserved_valueT; [exact Heq1| |]; eauto; ii; des).
-    clarify.
-    exploit IHvts; eauto; []; ii; des.
-    clarify.
-  - (exploit clear_unary_preserved_valueT; [exact Heq0| |]; eauto; ii; des).
-    exploit IHvts; eauto; []; ii; des.
-    clarify.
-Qed.
-
-Lemma clear_unary_preserved_expr
-      conf_unary st_unary invst_unary expr val f
-      (VAL: InvState.Unary.sem_expr conf_unary st_unary invst_unary expr = Some val)
-      (PRESERVED: List.forallb f (Exprs.Expr.get_idTs expr)):
-  <<VAL: InvState.Unary.sem_expr conf_unary st_unary (clear_unary f invst_unary) expr = Some val>>.
-Proof.
-  red.
-  unfold Exprs.Expr.get_idTs in *.
-  eapply forallb_filter_map in PRESERVED. des.
-  unfold is_true in PRESERVED. (* des_bool should kill it!!!!!!! KILL ALL is_true *)
-
-  Ltac exploit_clear_unary_preserved_with x :=
-    match (type of x) with
-    | (InvState.Unary.sem_valueT _ _ (clear_unary _ _) _ = _) => fail 1
-    | (InvState.Unary.sem_list_valueT _ _ (clear_unary _ _) _ = _) => fail 1
-    (* Above is REQUIRED in order to prevent inf loop *)
-    | (InvState.Unary.sem_valueT _ _ _ _ = Some _) =>
-      (exploit clear_unary_preserved_valueT; [exact x| |]; eauto; ii; des)
-    | (InvState.Unary.sem_list_valueT _ _ _ _ = Some _) =>
-      (exploit clear_unary_preserved_list_valueT; [exact x| |]; eauto; ii; des)
-    end.
-
-  Time destruct expr; ss;
-    repeat (des_bool; des); des_ifs; clarify;
-      (all_once exploit_clear_unary_subset_with); clarify;
-        (all_once exploit_clear_unary_preserved_with); clarify.
-Qed.
-
-Lemma incl_implies_preserved
-      conf st invst0 expr val inv
-      (preserved: _ -> bool)
-      (PRESERVED: forall id (ID: In id (Hints.Invariant.get_idTs_unary inv)), preserved id)
-      (VAL: InvState.Unary.sem_expr conf st invst0 expr = Some val)
-      (INCL: incl (Exprs.Expr.get_idTs expr) (Hints.Invariant.get_idTs_unary inv)):
-  <<PRESERVED: InvState.Unary.sem_expr conf st
-                                       (clear_unary preserved invst0)
-                                       expr = Some val>>.
-Proof.
-  eapply clear_unary_preserved_expr; eauto. apply forallb_forall. i.
-  apply PRESERVED. apply INCL. ss.
-Qed.
-
-Lemma clear_unary_spec
-      conf st invst invmem inv
-      (preserved: _ -> bool)
-      (PRESERVED: forall id (ID: In id (Hints.Invariant.get_idTs_unary inv)), preserved id)
-      (STATE: InvState.Unary.sem conf st invst invmem inv):
-  InvState.Unary.sem conf st
-                     (clear_unary preserved invst)
-                     invmem inv.
-Proof.
-  inv STATE. econs.
-  - ii.
-    exploit clear_unary_subset_expr; eauto. i. des.
-    exploit LESSDEF; eauto. i. des.
-    exploit incl_implies_preserved; eauto.
-    eapply incl_tran; [|eapply incl_tran].
-    + apply incl_appr. apply incl_refl.
-    + eapply In_list in H. des. refine H.
-    + unfold Hints.Invariant.get_idTs_unary.
-      apply incl_appl. apply incl_refl.
-  - inv NOALIAS. econs; i.
-    + eapply DIFFBLOCK; eauto.
-      * eapply clear_unary_subset_valueT; eauto.
-      * eapply clear_unary_subset_valueT; eauto.
-    + eapply NOALIAS0; eauto.
-      * eapply clear_unary_subset_valueT; eauto.
-      * eapply clear_unary_subset_valueT; eauto.
-  - ii. exploit UNIQUE; eauto. i. inv x0.
-    econs; eauto.
-  - ii. exploit PRIVATE; eauto.
-    eapply clear_unary_subset_idT; eauto.
 Qed.
 
 Lemma reduce_maydiff_non_physical_sound
@@ -357,25 +127,27 @@ Lemma reduce_maydiff_non_physical_sound
     <<STATE: InvState.Rel.sem conf_src conf_tgt st_src st_tgt invst1 invmem
                               (reduce_maydiff_non_physical inv)>>.
 Proof.
-  exists (clear_rel (reduce_maydiff_preserved inv) invst0). red.
-  inv STATE. econs; ss; cycle 2.
+  exists (InvState.Rel.filter (reduce_maydiff_preserved inv) invst0). red.
+  inv STATE.
+  econs; ss; cycle 2.
   - ii. ss.
     rewrite Exprs.IdTSetFacts.filter_b in NOTIN; [|solve_compat_bool].
     des_bool. des.
     + exploit MAYDIFF; eauto.
-      { exploit clear_unary_subset_idT; eauto. }
+      { exploit InvState.Unary.filter_subset_idT; eauto. }
       i. des. esplits; eauto.
       eapply reduce_maydiff_preserved_sem_idT; eauto.
     + destruct id0.
       rename t into __t__, i0 into __i__.
       unfold InvState.Unary.sem_idT in VAL_SRC. ss.
       unfold InvState.Unary.sem_tag in VAL_SRC. ss.
+      unfold compose in *.
       destruct __t__; inv NOTIN.
-      * rewrite clear_locals_spec in VAL_SRC.
+      * rewrite lookup_AL_filter_spec in VAL_SRC.
         unfold Exprs.Tag.t in *. rewrite H0 in VAL_SRC. ss.
-      * rewrite clear_locals_spec in VAL_SRC.
+      * rewrite lookup_AL_filter_spec in VAL_SRC.
         unfold Exprs.Tag.t in *. rewrite H0 in VAL_SRC. ss.
-  - apply clear_unary_spec; ss. i.
+  - apply InvState.Unary.filter_spec; ss. i.
     unfold reduce_maydiff_preserved. apply orb_true_iff. right.
     rewrite find_app.
     match goal with
@@ -385,7 +157,7 @@ Proof.
     end; ss.
     eapply find_none in COND; [|eauto].
     destruct (Exprs.IdT.eq_dec id0 id0); ss.
-  - apply clear_unary_spec; ss. i.
+  - apply InvState.Unary.filter_spec; ss. i.
     unfold reduce_maydiff_preserved. apply orb_true_iff. right.
     rewrite find_app.
     match goal with
